wip: list rules with georg and olivier

ErasedList.v
@@ -3,8 +3,10 @@ Require Export SystemFR.ErasedRecGen.
 Require Export SystemFR.ErasedSum.
 Require Export SystemFR.ErasedPair.
 Require Export SystemFR.ErasedTop.
+Require Export SystemFR.ErasedTypeRefine.
 
 Opaque strictly_positive.
+Opaque reducible_values.
 
 Lemma open_reducible_nil:
   forall tvars gamma,
@@ -20,10 +22,40 @@ Proof.
   apply open_reducible_unit.
 Qed.
 
+Lemma open_reducible_singleton:
+  forall tvars gamma t,
+    is_erased_term t ->
+    wf t 0 ->
+    subset (fv t) (support gamma) ->
+    [ tvars; gamma ⊨ t : T_top ] ->
+    [ tvars; gamma ⊨ t : tsingleton t ].
+Proof.
+  intros.
+  unfold tsingleton.
+  apply open_reducible_type_refine with uu;
+    repeat step || rewrite pfv_shift2 ||
+           unfold open_reducible ||
+           simp_red ||
+           apply reducible_value_expr ||
+           (rewrite shift_nothing2 by auto) ||
+           (rewrite open_none by auto);
+    eauto with erased wf fv;
+    try solve [ apply equivalent_refl; t_closer ].
+Qed.
+
+Lemma open_reducible_nil2:
+  forall tvars gamma,
+    [ tvars; gamma ⊨ tnil : Nil ].
+Proof.
+  intros.
+  apply open_reducible_singleton; steps; eauto with sets;
+    eauto using open_reducible_nil, open_reducible_top.
+Qed.
+
 Lemma open_reducible_cons:
-  forall tvars gamma h t T,
+  forall tvars gamma h t H,
+    [ tvars; gamma ⊨ h : H ] ->
     [ tvars; gamma ⊨ t : List ] ->
-    [ tvars; gamma ⊨ h : T ] ->
     [ tvars; gamma ⊨ tcons h t : List ].
 Proof.
   intros.
@@ -37,3 +69,91 @@ Proof.
     repeat step; eauto with sets;
     eauto using open_reducible_top.
 Qed.
+
+Lemma open_reducible_exists:
+  forall tvars gamma A B t a,
+    is_erased_type B ->
+    wf B 1 ->
+    subset (fv B) (support gamma) ->
+    [ tvars; gamma ⊨ a: A ] ->
+    [ tvars; gamma ⊨ t: open 0 B a ] ->
+    [ tvars; gamma ⊨ t: T_exists A B ].
+Proof.
+  unfold open_reducible;
+    repeat step || t_instantiate_sat3.
+
+  unfold reducible, reduces_to; steps; t_closer.
+
+  unfold reducible, reduces_to in H7; steps.
+
+  exists v; repeat step || simp_red; t_closer.
+
+  unfold reducible, reduces_to in H6; steps.
+
+  exists v0; repeat step || t_substitutions; t_closer.
+
+  eapply reducibility_values_ltr; eauto; steps; t_closer.
+Qed.
+
+Lemma open_reducible_cons2:
+  forall tvars gamma h t H T,
+    is_erased_type T ->
+    wf T 0 ->
+    subset (fv T) (support gamma) ->
+    is_erased_term h ->
+    wf h 0 ->
+    subset (fv h) (support gamma) ->
+    is_erased_term t ->
+    wf t 0 ->
+    subset (fv t) (support gamma) ->
+    [ tvars; gamma ⊨ h : H ] ->
+    [ tvars; gamma ⊨ t : T ] ->
+    [ tvars; gamma ⊨ tcons h t : Cons H T ].
+Proof.
+  unfold Cons; repeat step.
+
+  apply open_reducible_exists with h;
+    repeat step || rewrite open_none in * by auto; t_closer.
+
+  apply open_reducible_exists with t;
+    repeat step ||
+           (rewrite open_none in * by eauto with wf);
+    t_closer.
+
+  apply open_reducible_type_refine with uu;
+    repeat step || rewrite pfv_shift2 ||
+           simp_red ||
+           (rewrite shift_nothing2 by auto) ||
+           (rewrite open_none by auto);
+    eauto with erased wf fv;
+    try solve [ apply equivalent_refl; t_closer ];
+    eauto 2 with sets;
+    eauto using open_reducible_cons, open_reducible_top.
+
+  - apply open_reducible_top with (T_sum T_unit (T_prod H T)).
+    apply open_reducible_right.
+    apply open_reducible_pp; try eassumption; eauto with wf.
+    rewrite open_none; auto.
+
+  - unfold open_reducible; repeat step || apply reducible_value_expr || simp_red.
+    apply equivalent_refl; t_closer.
+Qed.
+
+Definition list_match t1 t2 t3 :=
+  sum_match t1 t2
+    (shift_open 0 (shift_open 1 t3 (pi1 (lvar 0 term_var))) (pi2 (lvar 0 term_var))).
+
+Lemma open_reducible_match:
+  forall tvars gamma t1 t2 t3 T1 T2 T3 x1 x2,
+    ~ x1 ∈ support gamma ->
+    ~ x2 ∈ support gamma ->
+    [ tvars; gamma ⊨ t1 : T1 ] ->
+    [ tvars; gamma ⊨ t2 : T2 ] ->
+    [ tvars; (x1, T_top) :: (x2, List) :: gamma ⊨
+        open 0 (open 1 t3 (fvar x1 term_var)) (fvar x2 term_var) :
+        open 0 (open 1 T3 (fvar x1 term_var)) (fvar x2 term_var) ] ->
+    [ tvars; gamma ⊨ list_match t1 t2 t3 : Match T1 T2 T3 ].
+Proof.
+  unfold list_match, Match;
+    repeat step.
+Admitted.
